backend/RenumberproofEFF.v
@@ -92,22 +92,6 @@ Proof.
   eapply function_ptr_translated; eauto.
 Qed.
 
-(*NEW, GFP as in selectionproofEFF*)
-Definition globalfunction_ptr_inject (j:meminj):=
-  forall b f, Genv.find_funct_ptr ge b = Some f -> 
-              j b = Some(b,0) /\ isGlobalBlock ge b = true.  
-
-Lemma restrict_preserves_globalfun_ptr: forall j X
-  (PG : globalfunction_ptr_inject j)
-  (Glob : forall b, isGlobalBlock ge b = true -> X b = true),
-globalfunction_ptr_inject (restrict j X).
-Proof. intros.
-  red; intros. 
-  destruct (PG _ _ H). split; trivial.
-  apply restrictI_Some; try eassumption.
-  apply (Glob _ H1).
-Qed.
-
 Lemma GDE_lemma: genvs_domain_eq ge tge.
 Proof.
     unfold genvs_domain_eq, genv2blocks.
@@ -117,38 +101,20 @@ Proof.
       exists id; assumption.
      rewrite symbols_preserved in Hid.
       exists id; assumption.
-     split; intros; destruct H as [id Hid].
-      rewrite <- varinfo_preserved in Hid.
-      exists id; assumption.
-     rewrite varinfo_preserved in Hid.
-      exists id; assumption.
-Qed.
-
-Lemma restrict_GFP_vis: forall mu
-  (GFP : globalfunction_ptr_inject (as_inj mu))
-  (Glob : forall b, isGlobalBlock ge b = true -> 
-                    frgnBlocksSrc mu b = true),
-  globalfunction_ptr_inject (restrict (as_inj mu) (vis mu)).
-Proof. intros.
-  unfold vis. 
-  eapply restrict_preserves_globalfun_ptr. eassumption.
-  intuition.
-Qed.
-
-(*From Cminorgenproof*)
-Remark val_inject_function_pointer:
-  forall v fd j tv,
-  Genv.find_funct ge v = Some fd ->
-  globalfunction_ptr_inject j ->
-  val_inject j v tv ->
-  tv = v.
-Proof.
-  intros. exploit Genv.find_funct_inv; eauto. intros [b EQ]. subst v.
-  inv H1.
-  rewrite Genv.find_funct_find_funct_ptr in H.
-  destruct (H0 _ _ H).
-  rewrite H1 in H4; inv H4.
-  rewrite Int.add_zero. trivial.
+     split; intros b. 
+       split; intros; destruct H as [id Hid].
+       rewrite <- varinfo_preserved in Hid.
+       exists id; assumption.
+       rewrite varinfo_preserved in Hid.
+       exists id; assumption.
+    intros. split.
+      intros [f H].
+        apply function_ptr_translated in H. 
+        eexists; eassumption.
+     intros [f H].
+         apply (@Genv.find_funct_ptr_rev_transf
+           _ _ _ transf_fundef prog) in H.
+         destruct H as [? [? _]]. eexists; eassumption.
 Qed.
 
 (** Effect of an injective renaming of nodes on a CFG. *)
@@ -217,7 +183,7 @@ Qed.
 Lemma regset_find_function_translated:
   forall j ros rs1 rs2 fd,
   meminj_preserves_globals ge j ->
-  globalfunction_ptr_inject j ->
+  globalfunction_ptr_inject ge j ->
   regset_inject j rs1 rs2 ->
   find_function ge ros rs1 = Some fd ->
   find_function tge ros rs2 = Some (transf_fundef fd).
@@ -333,10 +299,9 @@ Definition MATCH mu c1 m1 c2 m2:Prop :=
   match_states (restrict_sm mu (vis mu)) c1 m1 c2 m2 /\
   REACH_closed m1 (vis mu) /\
   meminj_preserves_globals ge (as_inj mu) /\
-  globalfunction_ptr_inject (as_inj mu) /\
+  globalfunction_ptr_inject ge (as_inj mu) /\
   (forall b, isGlobalBlock ge b = true -> frgnBlocksSrc mu b = true) /\
   sm_valid mu m1 m2 /\ SM_wd mu /\ Mem.inject (as_inj mu) m1 m2.
-
 
 (*Lenb: as in LinearizeproofEFF.v*)
 Lemma MATCH_wd: forall mu c1 m1 c2 m2 
