backend/SelectionproofEFF.v
@@ -2273,13 +2273,16 @@ Lemma MATCH_init_cores: forall v
   (Inj: Mem.inject j m1 m2)
   (VInj: Forall2 (val_inject j) vals1 vals2)
   (PG: meminj_preserves_globals ge j)
+  (R : list_norepet (map fst (prog_defs prog)))
   (J: forall b1 b2 d, j b1 = Some (b2, d) -> 
                       DomS b1 = true /\ DomT b2 = true)
   (RCH: forall b, REACH m2
         (fun b' : Values.block => isGlobalBlock tge b' || getBlocks vals2 b') b =
          true -> DomT b = true)
+  (InitMem : exists m0 : mem, Genv.init_mem prog = Some m0 
+               /\ Ple (Mem.nextblock m0) (Mem.nextblock m1) 
+               /\ Ple (Mem.nextblock m0) (Mem.nextblock m2))
   (GDE: genvs_domain_eq ge tge)
-  (GFP: globalfunction_ptr_inject ge j)
   (HDomS: forall b : Values.block, DomS b = true -> Mem.valid_block m1 b)
   (HDomT: forall b : Values.block, DomT b = true -> Mem.valid_block m2 b),
 exists c2 : CMinSel_core,
@@ -2378,10 +2381,15 @@ Proof. intros.
     apply BB.
     apply EE.
     rewrite initial_SM_as_inj.
-    red; intros. 
-    destruct PG as [X [Y Z]].
-    solve[eapply GFP; eauto].
-    rewrite initial_SM_as_inj. assumption. 
+      red; intros. specialize (Genv.find_funct_ptr_not_fresh prog). intros FFP.
+         destruct InitMem as [m0 [InitMem [? ?]]].
+         specialize (FFP _ _ _ InitMem H). 
+         destruct (valid_init_is_global _ R _ InitMem _ FFP) as [id Hid]. 
+           destruct PG as [PGa [PGb PGc]]. split. eapply PGa; eassumption.
+         unfold isGlobalBlock. 
+          apply orb_true_iff. left. apply genv2blocksBool_char1.
+            simpl. exists id; eassumption.
+    rewrite initial_SM_as_inj; assumption.
 Qed.
 
 Lemma MATCH_AfterExternal: 
@@ -3416,7 +3424,8 @@ Qed.
 
 Theorem transl_program_correct:
   forall (TRANSL: sel_program prog = OK tprog)
-         (R: list_norepet (map fst (prog_defs prog))),
+         (R: list_norepet (map fst (prog_defs prog)))
+         (init_mem: exists m0, Genv.init_mem prog = Some m0),
 SM_simulation.SM_simulation_inject (cmin_eff_sem hf)
    (cminsel_eff_sem hf) ge tge.
 Proof.
@@ -3438,7 +3447,50 @@ eapply effect_simulations_lemmas.inj_simulation_star with
   apply Match_genv.
 (*initial_core*)
   { intros.
-    apply (MATCH_init_cores _ _ _); eauto. }
+    apply (MATCH_init_cores _ _ _); eauto.
+    destruct init_mem as [m0 INIT].
+    exists m0; split; auto.
+    unfold meminj_preserves_globals in H2.    
+    destruct H2 as [A [B C]].
+
+    assert (P: forall p q, {Ple p q} + {Plt q p}).
+      intros p q.
+      case_eq (Pos.leb p q).
+      intros TRUE.
+      apply Pos.leb_le in TRUE.
+      left; auto.
+      intros FALSE.
+      apply Pos.leb_gt in FALSE.
+      right; auto.
+
+    cut (forall b, Plt b (Mem.nextblock m0) -> 
+           exists id, Genv.find_symbol ge id = Some b). intro D.
+    
+    split.
+    destruct (P (Mem.nextblock m0) (Mem.nextblock m1)); auto.
+    exfalso. 
+    destruct (D _ p).
+    apply A in H2.
+    assert (Mem.valid_block m1 (Mem.nextblock m1)).
+      eapply Mem.valid_block_inject_1; eauto.
+    clear - H7; unfold Mem.valid_block in H7.
+    xomega.
+
+    destruct (P (Mem.nextblock m0) (Mem.nextblock m2)); auto.
+    exfalso. 
+    destruct (D _ p).
+    apply A in H2.
+    assert (Mem.valid_block m2 (Mem.nextblock m2)).
+      eapply Mem.valid_block_inject_2; eauto.
+    clear - H7; unfold Mem.valid_block in H7.
+    xomega.
+    
+    intros b LT.    
+    unfold ge. 
+    apply valid_init_is_global with (b0 := b) in INIT.
+    eapply INIT; auto.
+    apply R.
+    apply LT. }
 (*halted*) 
   { intros. destruct H as [MC [RC [PG [GFP [GF [VAL [WD INJ]]]]]]]. 
     destruct c1; inv H0. destruct k; inv H1.
